Class for buffers and pointers (almost done)
***NO_CI***

ulib/FStar.BufferNG.fst
@@ -1203,6 +1203,14 @@ let disjoint_includes_l_swap #a #as #a' (x:pointer a) (subx:pointer as) (y:point
   [SMTPatT (disjoint y subx); SMTPatT (includes x subx)]
   = ()
 
+(*
+let disjoint_includes_r #a #as #a' (x: pointer a) (subx:pointer as) (y:pointer a') : Lemma
+  (requires (includes x subx /\ disjoint y x))
+  (ensures  (disjoint y subx))
+  [SMTPat (disjoint y subx); SMTPatT (includes x subx)]
+  = disjoint_includes x y subx y
+*)
+
 let live_disjoint
   (#value1: Type)
   (#value2: Type)
@@ -1729,9 +1737,9 @@ abstract let pointer_of_buffer_cell_disjoint
   [SMTPat (disjoint (pointer_of_buffer_cell b i1) (pointer_of_buffer_cell b i2))]
 = ()
 
-(* For a "disjoint" clause on buffers, we could use the following TRANSPARENT definitions: *)
+(* For a "disjoint" clause on buffers, we could use the following definitions: *)
 
-unfold
+abstract
 let disjoint_buffer_vs_pointer
   (#t1 #t2: Type)
   (b: buffer t1)
@@ -1739,7 +1747,7 @@ let disjoint_buffer_vs_pointer
 : GTot Type0
 = forall (i: UInt32.t { UInt32.v i < UInt32.v (buffer_length b) } ) . disjoint (pointer_of_buffer_cell b i) p
 
-unfold
+abstract
 let disjoint_buffer_vs_buffer
   (#t1 #t2: Type)
   (b1: buffer t1)
@@ -1750,6 +1758,80 @@ let disjoint_buffer_vs_buffer
     (i2: UInt32.t { UInt32.v i2 < UInt32.v (buffer_length b2) } )
   . 
     disjoint (pointer_of_buffer_cell b1 i1) (pointer_of_buffer_cell b2 i2) 
+
+let disjoint_buffer_vs_buffer_sym
+  (#t1 #t2: Type)
+  (b1: buffer t1)
+  (b2: buffer t2)
+: Lemma
+  (requires True)
+  (ensures (disjoint_buffer_vs_buffer b1 b2 <==> disjoint_buffer_vs_buffer b2 b1))
+  [SMTPat (disjoint_buffer_vs_buffer b1 b2)]
+= ()
+
+let disjoint_buffer_vs_pointer_singleton_buffer_of_pointer
+  (#t1 #t2: Type)
+  (b: pointer t1)
+  (p: pointer t2)
+: Lemma
+  (requires (disjoint b p))
+  (ensures (disjoint_buffer_vs_pointer (singleton_buffer_of_pointer b) p))
+  [SMTPat (disjoint_buffer_vs_pointer (singleton_buffer_of_pointer b) p)]
+= ()
+
+let disjoint_buffer_vs_buffer_singleton_buffer_of_pointer
+  (#t1 #t2: Type)
+  (b: buffer t1)
+  (p: pointer t2)
+: Lemma
+  (requires (disjoint_buffer_vs_pointer b p))
+  (ensures (disjoint_buffer_vs_buffer b (singleton_buffer_of_pointer p)))
+  [SMTPat (disjoint_buffer_vs_buffer b (singleton_buffer_of_pointer p))]
+= ()
+
+let disjoint_buffer_vs_pointer_buffer_of_array_pointer
+  (#len: UInt32.t)
+  (#t1 #t2: Type)
+  (b: pointer (array len t1))
+  (p: pointer t2)
+: Lemma
+  (requires (disjoint b p))
+  (ensures (disjoint_buffer_vs_pointer (buffer_of_array_pointer b) p))
+  [SMTPat (disjoint_buffer_vs_pointer (buffer_of_array_pointer b) p)]
+= assert (forall i . includes b (gcell b i))
+
+let disjoint_buffer_vs_buffer_buffer_of_array_pointer
+  (#len: UInt32.t)
+  (#t1 #t2: Type)
+  (b: buffer t1)
+  (p: pointer (array len t2))
+: Lemma
+  (requires (disjoint_buffer_vs_pointer b p))
+  (ensures (disjoint_buffer_vs_buffer b (buffer_of_array_pointer p)))
+  [SMTPat (disjoint_buffer_vs_buffer b (buffer_of_array_pointer p))]
+= assert (forall i . includes p (gcell p i))
+
+let disjoint_buffer_vs_buffer_pointer_of_buffer_cell
+  (#t1 #t2: Type)
+  (b1: buffer t1)
+  (b2: buffer t2)
+  (i: UInt32.t { UInt32.v i < UInt32.v (buffer_length b2) } )
+: Lemma
+  (requires (disjoint_buffer_vs_buffer b1 b2))
+  (ensures (disjoint_buffer_vs_pointer b1 (pointer_of_buffer_cell b2 i)))
+  [SMTPat (disjoint_buffer_vs_pointer b1 (pointer_of_buffer_cell b2 i))]
+= ()
+
+let disjoint_buffer_vs_pointer_pointer_of_buffer_cell
+  (#t1 #t2: Type)
+  (b: buffer t1)
+  (p: pointer t2)
+  (i: UInt32.t { UInt32.v i < UInt32.v (buffer_length b) } )
+: Lemma
+  (requires (disjoint_buffer_vs_pointer b p))
+  (ensures (disjoint (pointer_of_buffer_cell b i) p))
+  [SMTPat (disjoint (pointer_of_buffer_cell b i) p)]
+= ()
 
 let bwrite
   (#t: Type)
@@ -1762,8 +1844,7 @@ let bwrite
     modifies_1 (pointer_of_buffer_cell b i) h h' /\
     Seq.index (buffer_as_seq h' b) (UInt32.v i) == v /\ (
       forall (j: UInt32.t {UInt32.v j < UInt32.v (buffer_length b) /\ UInt32.v j <> UInt32.v i }) .
-        Seq.index (buffer_as_seq h' b) (UInt32.v j) == Seq.index (buffer_as_seq h b) (UInt32.v j)
-    
+        Seq.index (buffer_as_seq h' b) (UInt32.v j) == Seq.index (buffer_as_seq h b) (UInt32.v j)    
   )))
 = write (pointer_of_buffer_cell b i) v
 
@@ -1851,6 +1932,16 @@ let ancestor_buffer_of_array_pointer
   [SMTPat (buffer_ancestor (buffer_of_array_pointer p) == pointer_ancestor p)]
 = ()
 
+let ancestor_pointer_of_buffer_cell
+  (#t: Type)
+  (b: buffer t)
+  (i: UInt32.t { UInt32.v i < UInt32.v (buffer_length b) } )
+: Lemma
+  (requires True)
+  (ensures (pointer_ancestor (pointer_of_buffer_cell b i) == buffer_ancestor b))
+  [SMTPat (pointer_ancestor (pointer_of_buffer_cell b i))]
+= ()
+
 let object_ancestor
   (o: object)
 : Tot HyperStack.object
@@ -1873,20 +1964,236 @@ let objects_disjoint
     | ObjectPointer p2 -> disjoint p1 p2
     end
 
-(*
+private
+let buffer_root_live
+  (#t: Type)
+  (h: HS.mem)
+  (b: buffer_root t)
+: Tot Type0
+= match b with
+  | BufferRootSingleton p -> live h p
+  | BufferRootArray p -> live h p
 
-let class': Modifies.class HyperStack.mem 1 object =
+abstract
+let buffer_live
+  (#t: Type)
+  (h: HS.mem)
+  (b: buffer t)
+: Tot Type0
+= buffer_root_live h (Buffer?.broot b)
+
+abstract
+let buffer_live_singleton_buffer_of_pointer
+  (#t: Type)
+  (h: HS.mem)
+  (p: pointer t)
+: Lemma
+  (requires True)
+  (ensures (buffer_live h (singleton_buffer_of_pointer p) == live h p))
+  [SMTPat (buffer_live h (singleton_buffer_of_pointer p))]
+= ()
+
+abstract
+let buffer_live_buffer_of_array_pointer
+  (#len: UInt32.t)
+  (#t: Type)
+  (h: HS.mem)
+  (p: pointer (array len t))
+: Lemma
+  (requires True)
+  (ensures (buffer_live h (buffer_of_array_pointer p) == live h p))
+  [SMTPat (buffer_live h (buffer_of_array_pointer p))]
+= ()
+
+abstract
+let live_pointer_of_buffer_cell
+  (#t: Type)
+  (h: HS.mem)
+  (b: buffer t)
+  (i: UInt32.t { UInt32.v i < UInt32.v (buffer_length b) } )
+: Lemma
+  (requires True)
+  (ensures (live h (pointer_of_buffer_cell b i) == buffer_live h b))
+  [SMTPat (live h (pointer_of_buffer_cell b i))]
+= ()
+
+let object_live
+  (h: HS.mem)
+  (o: object)
+= match o with
+  | ObjectBuffer b -> buffer_live h b
+  | ObjectPointer p -> live h p
+
+private
+let buffer_root_contains
+  (#t: Type)
+  (h: HS.mem)
+  (b: buffer_root t)
+: Tot Type0
+= match b with
+  | BufferRootSingleton p -> contains h p
+  | BufferRootArray p -> contains h p
+
+abstract
+let buffer_contains
+  (#t: Type)
+  (h: HS.mem)
+  (b: buffer t)
+: Tot Type0
+= buffer_root_contains h (Buffer?.broot b)
+
+abstract
+let buffer_contains_singleton_buffer_of_pointer
+  (#t: Type)
+  (h: HS.mem)
+  (p: pointer t)
+: Lemma
+  (requires True)
+  (ensures (buffer_contains h (singleton_buffer_of_pointer p) == contains h p))
+  [SMTPat (buffer_contains h (singleton_buffer_of_pointer p))]
+= ()
+
+abstract
+let buffer_contains_buffer_of_array_pointer
+  (#len: UInt32.t)
+  (#t: Type)
+  (h: HS.mem)
+  (p: pointer (array len t))
+: Lemma
+  (requires True)
+  (ensures (buffer_contains h (buffer_of_array_pointer p) == contains h p))
+  [SMTPat (buffer_contains h (buffer_of_array_pointer p))]
+= ()
+
+abstract
+let contains_pointer_of_buffer_cell
+  (#t: Type)
+  (h: HS.mem)
+  (b: buffer t)
+  (i: UInt32.t { UInt32.v i < UInt32.v (buffer_length b) } )
+: Lemma
+  (requires True)
+  (ensures (contains h (pointer_of_buffer_cell b i) == buffer_contains h b))
+  [SMTPat (contains h (pointer_of_buffer_cell b i))]
+= ()
+
+let object_contains
+  (h: HS.mem)
+  (o: object)
+= match o with
+  | ObjectBuffer b -> buffer_contains h b
+  | ObjectPointer p -> contains h p
+
+abstract
+let pointer_preserved
+  (#t: Type)
+  (p: pointer t)
+  (h1 h2: HS.mem)
+: Tot Type0
+= (live h1 p ==> (live h2 p /\ gread h2 p == gread h1 p))
+
+abstract
+let buffer_preserved
+  (#t: Type)
+  (p: buffer t)
+  (h1 h2: HS.mem)
+: Tot Type0
+= (buffer_live h1 p ==> (buffer_live h2 p /\ buffer_as_seq h2 p == buffer_as_seq h1 p))
+
+let object_preserved
+  (o: object)
+  (h1 h2: HS.mem)
+: Tot Type0
+= match o with
+  | ObjectBuffer b -> buffer_preserved b h1 h2
+  | ObjectPointer p -> pointer_preserved p h1 h2
+
+let class': Modifies.class' HS.mem 1 object =
   Modifies.Class
-    (* heap  *)                 mem
+    (* heap  *)                 HS.mem
     (* level *)                 1
     (* carrier *)               object
     (* disjoint *)              objects_disjoint
     (* live *)                  object_live
     (* contains *)              object_contains
     (* preserved *)             object_preserved
-    (* ancestor_count *)        (fun x -> 0)
-    (* ancestor_types *)        (fun x y -> false_elim ())
-    (* ancestor_class_levels *) (fun x y -> false_elim ())
-    (* ancestor_classes *)      (fun x y -> false_elim ())
-    (* ancestor_objects *)      (fun x y -> false_elim ())
-  
+    (* ancestor_count *)        (fun x -> 1)
+    (* ancestor_types *)        (fun x y -> HS.object)
+    (* ancestor_class_levels *) (fun x y -> 0)
+    (* ancestor_classes *)      (fun x y -> HS.class)
+    (* ancestor_objects *)      (fun x y -> object_ancestor x)
+
+abstract
+let class_invariant ()
+: Lemma 
+  (requires True)
+  (ensures (Modifies.class_invariant HS.class class'))
+  [SMTPat (Modifies.class_invariant HS.class class')]
+= let s: Modifies.class_invariant_body u#0 u#1 HS.class class' = {
+    Modifies.preserved_refl = (let f _ _ = () in f);
+    Modifies.preserved_trans = (let f _ _ _ _ = () in f);
+    Modifies.preserved_ancestors_preserved = begin
+      let g
+	(x: object)
+	(h: HS.mem)
+	(h' : HS.mem)
+	(s: squash (Modifies.Class?.ancestor_count class' x > 0))
+	(f: (
+	  (i: nat { i < Modifies.Class?.ancestor_count class' x } ) ->
+	  Lemma
+	  (Modifies.Class?.preserved (Modifies.Class?.ancestor_classes class' x i) (Modifies.ancestor_objects class' x i) h h')
+	))
+      : Lemma
+	(ensures (Modifies.Class?.preserved class' x h h'))
+      = f 0
+      in
+      g
+    end;
+    Modifies.class_disjoint_sym = (let f _ _ = () in f);
+    Modifies.level_0_class_eq_root = ();
+    Modifies.level_0_fresh_disjoint = (let f _ _ _ _ = () in f);
+    Modifies.preserved_live = (let f _ _ _ = () in f);
+    Modifies.preserved_contains = (let f _ _ _ = () in f);
+    Modifies.live_contains = (let f _ _ = () in f);
+    Modifies.ancestors_contains = begin
+      let g
+	(h: HS.mem)
+	(o: object)
+	(s: squash (Modifies.Class?.ancestor_count class' o > 0))
+	(f: (
+	  (i: nat {i < Modifies.Class?.ancestor_count class' o } ) ->
+	  Lemma
+	  (Modifies.Class?.contains (Modifies.Class?.ancestor_classes class' o i) h (Modifies.ancestor_objects class' o i))
+        ))
+      : Lemma
+	(ensures (Modifies.Class?.contains class' h o))
+      = f 0
+      in
+      g
+    end;
+    Modifies.live_ancestors = (let f _ _ _ = () in f)
+  }
+  in
+  (Modifies.class_invariant_intro s)
+
+let class: Modifies.class HS.class 1 object = class'
+
+let class_eq
+  ()
+: Lemma
+  (requires True)
+  (ensures (class == class'))
+  [SMTPatOr [[SMTPat class]; [SMTPat class']]]
+= ()
+
+let singleton_pointer
+  (#t: Type)
+  (p: pointer t)
+: Tot (TSet.set (Modifies.object HS.class))
+= Modifies.singleton class (ObjectPointer p)
+
+let singleton_buffer
+  (#t: Type)
+  (b: buffer t)
+: Tot (TSet.set (Modifies.object HS.class))
+= Modifies.singleton class (ObjectBuffer b)
